\textbf{\textcolor{blue}{2.}} \Large
Aplica $\alpha$-conversiones en cada expresión
para cambiar los términos de las variables de ligado.
\begin{enumerate}[a)]
%%%%%%%%%%%%%%%%%%%%%%%%      Inciso a    %%%%%%%%%%%%%%%%%%%%%%%%%%%%
    \item $\lambda a.\lambda b.(\lambda a.b \; \lambda b.a)$
    
    \textbf{Solución:}
    \begin{eqnarray*}
        \lambda_a . \lambda_b . (\lambda_a . b \; \lambda_b . a)
        \rightarrow_{\alpha} \lambda_x . \lambda_y (\lambda_z . y \lambda_w z)
    \end{eqnarray*}
%%%%%%%%%%%%%%%%%%%%%%%%      Inciso b    %%%%%%%%%%%%%%%%%%%%%%%%%%%%
    \item $\lambda a.(a(\lambda b.(\lambda a.a\; b)a))$
    
    \textbf{Solución:}
    \begin{eqnarray*}
        \lambda_a .(a(\lambda_b .(\lambda_a .a\; b)a))
        \rightarrow_{\alpha} \lambda_x .(x(\lambda_y .(\lambda_w .w\; y)x))
    \end{eqnarray*}
%%%%%%%%%%%%%%%%%%%%%%%%      Inciso c    %%%%%%%%%%%%%%%%%%%%%%%%%%%%
    \item $\lambda x.(\lambda y.x\; \lambda y.(\lambda x.x \; y))$
    
    \textbf{Solución:}
    \begin{eqnarray*}
        \lambda_x .(\lambda_y .x\; \lambda_y .(\lambda_x .x \; y))
        \rightarrow_{\alpha} \lambda_a .(\lambda_b .a\; \lambda_c .(\lambda_e .e \; c))
    \end{eqnarray*}
\end{enumerate}
